thys/LLL_Basis_Reduction/LLL_Complexity.thy
@@ -147,7 +147,7 @@ definition basis_reduction_add_rows_cost :: "state \<Rightarrow> state cost" whe
         gjs = fst G
       in basis_reduction_add_row_i_all_main_cost state fjs gjs)" 
 
-lemma basis_reduction_add_rows_cost: assumes "LLL_invariant state F G" 
+lemma basis_reduction_add_rows_cost: assumes "LLL_invariant outside state F G" 
   shows "result (basis_reduction_add_rows_cost state) = basis_reduction_add_rows state" (is ?g1)
      "cost (basis_reduction_add_rows_cost state) \<le> 4 * m * n * arith_cost" (is ?g2)
 proof -
@@ -171,7 +171,7 @@ definition basis_reduction_step_cost :: "state \<Rightarrow> state cost" where
 
 definition "body_cost = (4 * m + 12) * n * arith_cost" 
 
-lemma basis_reduction_step_cost: assumes "LLL_invariant state F G" 
+lemma basis_reduction_step_cost: assumes "LLL_invariant outside state F G" 
   shows "result (basis_reduction_step_cost state) = basis_reduction_step \<alpha> state" (is ?g1)
      "cost (basis_reduction_step_cost state) \<le> body_cost" (is ?g2)
 proof -
@@ -193,7 +193,7 @@ qed
 function basis_reduction_main_cost :: "state \<Rightarrow> state cost" where
   "basis_reduction_main_cost state = (
      case state of (i,F,G) \<Rightarrow>
-     if i < m \<and> (\<exists> FF GG. LLL_invariant state FF GG) 
+     if i < m \<and> (\<exists> FF GG. LLL_invariant True state FF GG) 
        \<comment> \<open>The check on the invariant is just to be able to prove termination. 
           One cannot use partial-function at this point, since the function with cost is not tail-recursive.\<close>
      then case basis_reduction_step_cost state of 
@@ -207,7 +207,7 @@ termination
 proof (standard, rule wf_measure[of LLL_measure], goal_cases)
   case (1 state i FG F G state1 c1)
   note * = 1(1)[symmetric] 1(2)[symmetric] 1(3) 1(4)[symmetric]
-  from * obtain FF GG where i: "i < m" and inv: "LLL_invariant (i, F, G) FF GG" by auto
+  from * obtain FF GG where i: "i < m" and inv: "LLL_invariant True (i, F, G) FF GG" by auto
   from basis_reduction_step_cost[OF inv, unfolded *] 
   have res: "basis_reduction_step \<alpha> (i, F, G) = state1" using * cost_simps(2) by metis
   from basis_reduction_step[OF inv i res]
@@ -218,17 +218,17 @@ declare basis_reduction_main_cost.simps[simp del]
 
 definition "num_loops = m + 2 * m * m * nat (ceiling (log base (real A)))"
 
-lemma basis_reduction_main_cost: fixes F G assumes "LLL_invariant state F G"
+lemma basis_reduction_main_cost: fixes F G assumes "LLL_invariant True state F G"
   shows "result (basis_reduction_main_cost state) = basis_reduction_main \<alpha> m state" (is ?g1) 
    "cost (basis_reduction_main_cost state) \<le> body_cost * num_loops" (is ?g2)
 proof -
-  have inv: "LLL_partial_invariant state F G" using assms unfolding LLL_invariant_def by auto
+  have inv: "LLL_invariant True state F G" using assms unfolding LLL_invariant_def by auto
   have ?g1 and cost: "cost (basis_reduction_main_cost state) \<le> body_cost * LLL_measure state"
     using assms
   proof (atomize (full), induct state arbitrary: F G rule: wf_induct[OF wf_measure[of LLL_measure]])
     case (1 state F G)
     note inv = 1(2)
-    have ex: "(\<exists>FF. Ex (LLL_invariant state FF)) = True" using inv by auto
+    have ex: "(\<exists>FF. Ex (LLL_invariant True state FF)) = True" using inv by auto
     note IH = 1(1)[rule_format]
     obtain i Fr1 Gr1 where state: "state = (i,Fr1,Gr1)" by (cases state, auto)
     note inv = inv[unfolded state]
@@ -246,7 +246,7 @@ proof -
       note simp = simp[unfolded rec split]
       from simp i have res: "basis_reduction_main_cost state = (state2, c1 + c2)" by auto    
       note bsr = basis_reduction_step[OF inv i bb]
-      from bsr(1) obtain F' G' where inv: "LLL_invariant state1 F' G'" by auto
+      from bsr(1) obtain F' G' where inv: "LLL_invariant True state1 F' G'" by auto
       from bsr(2) have "(state1 ,state) \<in> measure LLL_measure" by (auto simp: state)
       from IH[OF this inv, unfolded rec cost_simps]
       have res': "basis_reduction_main \<alpha> m state1 = state2" 
@@ -396,7 +396,7 @@ proof -
   from initial_state_cost[unfolded init cost_simps]
   have c1: "c1 \<le> initial_gso_cost" and init: "initial_state n fs_init = state1" by auto
   from initial_state[OF init]
-  obtain F' G' where inv: "LLL_invariant state1 F' G'" by auto
+  obtain F' G' where inv: "LLL_invariant True state1 F' G'" by auto
   from basis_reduction_main_cost[OF inv, unfolded main cost_simps]
   have main: "basis_reduction_main \<alpha> m state1 = state2" and c2: "c2 \<le> body_cost * num_loops" 
     by auto
